Extra laws for Circus while loops

theories/sf_rdes/utp_sfrd_healths.thy
@@ -683,12 +683,15 @@ qed (simp_all)
 abbreviation TestC ("test\<^sub>C") where
 "test\<^sub>C P \<equiv> csp_theory.utp_test P"
 
-abbreviation StarC :: "('\<sigma>, '\<phi>) action \<Rightarrow> ('\<sigma>, '\<phi>) action" ("_\<^sup>\<star>\<^sup>C" [999] 999) where
+definition StarC :: "('\<sigma>, '\<phi>) action \<Rightarrow> ('\<sigma>, '\<phi>) action" ("_\<^sup>\<star>\<^sup>C" [999] 999) where
 "StarC P \<equiv> csp_theory.utp_star P"
+
+lemma StarC_unfold: "P is NCSP \<Longrightarrow> P\<^sup>\<star>\<^sup>C = Skip \<sqinter> (P ;; P\<^sup>\<star>\<^sup>C)"
+  by (simp add: StarC_def csp_theory.Star_unfoldl_eq)
 
 lemma sfrd_star_as_rdes_star:
   "P is NCSP \<Longrightarrow> P\<^sup>\<star>\<^sup>C = P\<^sup>\<star>\<^sup>R ;; Skip"
-  by (simp add: csp_theory.Star_alt_def nsrdes_theory.Star_alt_def StarR_def closure unrest Skip_srdes_left_unit csp_theory.Unit_Right)
+  by (simp add: StarC_def csp_theory.Star_alt_def nsrdes_theory.Star_alt_def StarR_def closure unrest Skip_srdes_left_unit csp_theory.Unit_Right)
 
 theorem csp_star_rdes_def [rdes_def]:
   assumes "P is CRC" "Q is CRR" "R is CRF" "$st\<acute> \<sharp> Q"
